Foundation/Modal/Neighborhood/AxiomGeach.lean
@@ -1,0 +1,74 @@
+import Foundation.Modal.Tableau
+import Foundation.Modal.Neighborhood.Basic
+
+namespace LO.Modal.Neighborhood
+
+open Formula (atom)
+open Formula.Neighborhood
+
+
+variable {F : Frame} {X Y : Set F.World} {g : Axioms.Geach.Taple}
+
+namespace Frame
+
+class IsGeachConvergent (g : Axioms.Geach.Taple) (F : Frame) : Prop where
+  gconv : ∀ X : Set F, 𝒟^[g.i] (ℬ^[g.m] X) ⊆ ℬ^[g.j] (𝒟^[g.n] X)
+
+@[simp, grind]
+lemma gconv [F.IsGeachConvergent g] : 𝒟^[g.i] (ℬ^[g.m] X) ⊆ ℬ^[g.j] (𝒟^[g.n] X) := IsGeachConvergent.gconv X
+
+
+class IsReflexive (F : Frame) : Prop where
+  refl : ∀ X : Set F, ℬ X ⊆ X
+
+@[simp, grind] lemma refl [F.IsReflexive] : ℬ X ⊆ X := IsReflexive.refl X
+
+instance [F.IsReflexive] : F.IsGeachConvergent ⟨0, 0, 1, 0⟩ := ⟨by simp⟩
+
+instance [F.IsGeachConvergent ⟨0, 0, 1, 0⟩] : F.IsReflexive := ⟨λ _ => F.gconv (g := ⟨0, 0, 1, 0⟩)⟩
+
+
+class IsTransitive (F : Frame) : Prop where
+  trans : ∀ X : Set F, ℬ X ⊆ ℬ^[2] X
+
+@[simp, grind] lemma trans [F.IsTransitive] : ℬ X ⊆ ℬ^[2] X := IsTransitive.trans X
+
+instance [F.IsTransitive] : F.IsGeachConvergent ⟨0, 2, 1, 0⟩ := ⟨by simp⟩
+
+instance [F.IsGeachConvergent ⟨0, 2, 1, 0⟩] : F.IsTransitive := ⟨λ _ => F.gconv (g := ⟨0, 2, 1, 0⟩)⟩
+
+end Frame
+
+
+section
+
+variable {a : ℕ}
+
+lemma valid_axiomGeach_of_isGeachConvergent [F.IsGeachConvergent g] : F ⊧ Axioms.Geach g (.atom a) := by
+  intro V x;
+  apply Satisfies.def_imp.mpr;
+  suffices x ∈ 𝒟^[g.i] (ℬ^[g.m] (V a)) → x ∈ ℬ^[g.j] (𝒟^[g.n] (V a)) by simpa [Semantics.Realize, Satisfies];
+  apply F.gconv;
+
+@[simp] lemma valid_axiomT_of_isReflexive [F.IsReflexive] : F ⊧ Axioms.T (.atom a) := valid_axiomGeach_of_isGeachConvergent (g := ⟨0, 0, 1, 0⟩)
+@[simp] lemma valid_axiomFour_of_isTransitive [F.IsTransitive] : F ⊧ Axioms.Four (.atom a) := valid_axiomGeach_of_isGeachConvergent (g := ⟨0, 2, 1, 0⟩)
+
+lemma isGeachConvergent_of_valid_axiomGeach (h : F ⊧ Axioms.Geach g (.atom a)) : F.IsGeachConvergent g := by
+  constructor;
+  intro X x hx;
+  have : x ∈ 𝒟^[g.i] (ℬ^[g.m] X) → x ∈ ℬ^[g.j] (𝒟^[g.n] X) := by
+    simpa [Semantics.Realize, Satisfies] using Satisfies.def_imp.mp $ @h (λ _ => X) x;
+  apply this;
+  apply hx;
+
+lemma isReflexive_of_valid_axiomT (h : F ⊧ Axioms.T (.atom a)) : F.IsReflexive := by
+  have := isGeachConvergent_of_valid_axiomGeach (g := ⟨0, 0, 1, 0⟩) h;
+  infer_instance;
+
+lemma isTransitive_of_valid_axiomFour (h : F ⊧ Axioms.Four (.atom a)) : F.IsTransitive := by
+  have := isGeachConvergent_of_valid_axiomGeach (g := ⟨0, 2, 1, 0⟩) h;
+  infer_instance;
+
+end
+
+end LO.Modal.Neighborhood
