Foundation/Modal/Neighborhood/Logic/EMCN.lean
@@ -23,17 +23,8 @@ namespace Hilbert
 namespace EMCN.Neighborhood
 
 instance : Sound Hilbert.EMCN FrameClass.EMCN := instSound_of_validates_axioms $ by
-  simp only [Semantics.RealizeSet.insert_iff, Semantics.RealizeSet.singleton_iff];
-  refine ⟨?_, ?_, ?_⟩;
-  . intro F hF;
-    replace hF := Set.mem_setOf_eq.mp hF;
-    apply valid_axiomM_of_isMonotonic;
-  . intro F hF;
-    replace hF := Set.mem_setOf_eq.mp hF;
-    apply valid_axiomC_of_isRegular;
-  . intro F hF;
-    replace hF := Set.mem_setOf_eq.mp hF;
-    apply valid_axiomN_of_ContainsUnit;
+  constructor;
+  rintro _ (rfl | rfl | rfl) F (rfl | rfl | rfl) <;> simp;
 
 instance : Entailment.Consistent Hilbert.EMCN := consistent_of_sound_frameclass FrameClass.EMCN $ by
   use Frame.simple_blackhole;
@@ -81,10 +72,7 @@ instance : Hilbert.ECN ⪱ Hilbert.EMCN := by
       apply not_validOnFrameClass_of_exists_model_world;
       let M : Model := {
         World := Fin 2,
-        𝒩 := λ w =>
-          match w with
-          | 0 => {∅, {0, 1}}
-          | 1 => {∅, {0, 1}},
+        𝒩 := λ w => {∅, {0, 1}},
         Val := λ w =>
           match w with
           | 0 => {0}
@@ -99,12 +87,10 @@ instance : Hilbert.ECN ⪱ Hilbert.EMCN := by
             match x with | 0 | 1 => simp_all [M, Set.Fin2.eq_univ];
           regular := by
             rintro X Y w ⟨hwX, hwY⟩;
-            match w with
-            | 0 | 1 =>
-              simp_all only [Fin.isValue, Set.mem_setOf_eq, Set.mem_insert_iff, Set.mem_singleton_iff, M];
-              rcases hwX with (rfl | rfl) <;>
-              rcases hwY with (rfl | rfl) <;>
-              simp;
+            simp_all only [Fin.isValue, Set.mem_setOf_eq, Set.mem_insert_iff, Set.mem_singleton_iff, M];
+            rcases hwX with (rfl | rfl) <;>
+            rcases hwY with (rfl | rfl) <;>
+            simp;
         }
       . simp! [M, Semantics.Realize, Satisfies];
         tauto_set;
