Foundation/Modal/Neighborhood/Logic/EMT.lean
@@ -1,0 +1,59 @@
+import Foundation.Modal.Neighborhood.Logic.EM
+import Foundation.Modal.Neighborhood.AxiomGeach
+
+namespace LO.Modal
+
+open Neighborhood
+open Hilbert.Neighborhood
+open Formula.Neighborhood
+
+namespace Neighborhood
+
+instance : Frame.simple_blackhole.IsReflexive := by
+  constructor;
+  intro X x;
+  simp_all;
+
+protected class Frame.IsEMT (F : Frame) extends F.IsMonotonic, F.IsReflexive
+protected abbrev FrameClass.EMT : FrameClass := { F | F.IsEMT }
+
+end Neighborhood
+
+
+namespace Hilbert
+
+namespace EMT.Neighborhood
+
+instance : Sound Hilbert.EMT FrameClass.EMT := instSound_of_validates_axioms $ by
+  constructor;
+  rintro _ (rfl | rfl) F (rfl | rfl) <;> simp;
+
+instance : Entailment.Consistent Hilbert.EMT := consistent_of_sound_frameclass FrameClass.EMT $ by
+  use Frame.simple_blackhole;
+  apply Set.mem_setOf_eq.mpr;
+  constructor;
+
+end EMT.Neighborhood
+
+instance : Hilbert.EM ⪱ Hilbert.EMT := by
+  constructor;
+  . apply Hilbert.WithRE.weakerThan_of_subset_axioms;
+    simp;
+  . apply Entailment.not_weakerThan_iff.mpr;
+    use (Axioms.T (.atom 0));
+    constructor;
+    . simp;
+    . apply Sound.not_provable_of_countermodel (𝓜 := FrameClass.EM);
+      apply not_validOnFrameClass_of_exists_frame;
+      use ⟨Fin 1, λ _ => Set.univ⟩;
+      constructor;
+      . exact ⟨by tauto⟩;
+      . apply not_imp_not.mpr isReflexive_of_valid_axiomT;
+        by_contra! hC;
+        simpa [Frame.box] using @hC.refl ∅;
+
+end Hilbert
+
+instance : 𝐄𝐌 ⪱ 𝐄𝐌𝐓 := inferInstance
+
+end LO.Modal
