Foundation/Modal/Neighborhood/Logic/EMT4.lean
@@ -1,0 +1,52 @@
+import Foundation.Modal.Neighborhood.Logic.EMT
+import Foundation.Modal.Neighborhood.Logic.E4
+
+namespace LO.Modal
+
+open Neighborhood
+open Hilbert.Neighborhood
+open Formula.Neighborhood
+
+namespace Neighborhood
+
+protected class Frame.IsEMT4 (F : Frame) extends F.IsMonotonic, F.IsReflexive, F.IsTransitive
+protected abbrev FrameClass.EMT4 : FrameClass := { F | F.IsEMT4 }
+
+end Neighborhood
+
+
+namespace Hilbert
+
+namespace EMT4.Neighborhood
+
+instance : Sound Hilbert.EMT4 FrameClass.EMT4 := instSound_of_validates_axioms $ by
+  constructor;
+  rintro _ (rfl | rfl | rfl) F (rfl | rfl) <;> simp;
+
+instance : Entailment.Consistent Hilbert.EMT4 := consistent_of_sound_frameclass FrameClass.EMT4 $ by
+  use Frame.simple_blackhole;
+  apply Set.mem_setOf_eq.mpr;
+  constructor;
+
+end EMT4.Neighborhood
+
+instance : Hilbert.EMT ⪱ Hilbert.EMT4 := by
+  constructor;
+  . apply Hilbert.WithRE.weakerThan_of_subset_axioms;
+    simp;
+  . apply Entailment.not_weakerThan_iff.mpr;
+    use (Axioms.Four (.atom 0));
+    constructor;
+    . simp;
+    . apply Sound.not_provable_of_countermodel (𝓜 := FrameClass.EMT);
+      apply not_validOnFrameClass_of_exists_frame;
+      use Frame.trivial_nontransitive;
+      constructor;
+      . constructor;
+      . simp;
+
+end Hilbert
+
+instance : 𝐄𝐌𝐓 ⪱ 𝐄𝐌𝐓𝟒 := inferInstance
+
+end LO.Modal
